src/PlutusIR/Semantics/SemanticEquivalence/CompatibilityLemmas/TyAbs.v
@@ -7,10 +7,126 @@ Require Import PlutusCert.PlutusIR.Semantics.TypeSafety.BaseKindedness.
 Require Import PlutusCert.PlutusIR.Semantics.TypeSafety.TypeLanguage.StrongNormalisation.
 Require Import PlutusCert.PlutusIR.Semantics.TypeSafety.TypeLanguage.Preservation.
 Require Import PlutusCert.PlutusIR.Semantics.SemanticEquivalence.Multisubstitution.Congruence.
+From PlutusCert Require Import SubstitutionPreservesTyping.
 
 Require Import Arith.
 
+Require Import PlutusCert.Util.Tactics.
+Require Import Lists.List.
 
+Lemma drop_ty_var__RG ρ k Γ γ γ' : forall bX,
+  RG ρ k Γ γ γ' ->
+    exists γ_dropped γ_dropped',
+      RG ρ k (drop_ty_var bX Γ) γ_dropped γ_dropped'.
+Proof.
+  induction 1.
+  - eexists nil, nil. eauto using RG.
+  - simpl.
+    destruct_hypos.
+    destruct_if.
+    + revert H_eqb. destruct_if.
+      * inversion 1.
+      * eauto using RG.
+    + revert H_eqb. destruct_if.
+      * intros _. eauto.
+      * inversion 1.
+Qed.
+
+Open Scope string_scope.
+Import ListNotations.
+
+Lemma drop_RG k Γ γ γ' x :
+  0 < k ->
+  RG [] k Γ γ γ' ->
+  RG [] k (drop x Γ) (drop x γ) (drop x γ')
+.
+Proof.
+  induction 2; simpl.
+  - constructor.
+  - destruct (x0 =? x);
+    eauto using RG.
+Qed.
+(*
+Lemma drop_RG_msubst k Γ γ γ' x :
+  0 < k ->
+  RG [] k Γ γ γ' ->
+    (forall t T, [] ,, drop x Γ |-+ t : T -> msubst γ t = msubst (drop x γ) t) /\
+    (forall t T, [] ,, drop x Γ |-+ t : T -> msubst γ' t = msubst (drop x γ') t)
+.
+Proof.
+  intros H_k.
+  induction 1.
+  - simpl. split; constructor.
+  - rewrite drop_equation.
+    simpl.
+    destruct (x0 =? x) eqn:Heq.
+    + (* x0 = x *)
+      apply eqb_eq in Heq. subst x0.
+      destruct_hypos.
+      split.
+      * eauto.
+      * split.
+        ** intros t T' H_ty.
+           specialize (H4 _ _ H_ty).
+           simpl.
+           rewrite <- H4.
+           assert (H_id : subst x v1 t = t) by admit. (* x not free in t *)
+           rewrite H_id. reflexivity.
+        ** intros t T' H_ty.
+           specialize (H5 _ _ H_ty).
+           simpl.
+           rewrite <- H5.
+           assert (H_id : subst x v2 t = t) by admit. (* x not free in t *)
+           rewrite H_id. reflexivity.
+    + (* x0 /= x *)
+      destruct_hypos.
+      eexists. eexists.
+      split.
+      * constructor; eauto.
+      * split.
+        ** intros t T' H_ty.
+           simpl.
+           eapply H4.
+           apply RV_typable_empty_1 in H.
+           destruct_hypos.
+           simpl in *.
+           eapply substitution_preserves_typing__Term.
+           *** eassumption.
+           *** eauto.
+           *** eauto.
+           *** eauto.
+        ** intros t T' H_ty.
+           simpl.
+           eapply H5.
+           apply RV_typable_empty_2 in H.
+           destruct_hypos.
+           simpl in *.
+           eapply substitution_preserves_typing__Term.
+           *** eassumption.
+           *** eauto.
+           *** eauto.
+           *** eauto.
+Admitted.
+*)
+
+Lemma approx_drop Δ x Γ e e' T :
+  Δ,, (drop x Γ) |- e ≤ e' : T ->
+  Δ,, Γ |- e ≤ e' : T.
+Proof.
+  intros H_approx_drop.
+  unfold LR_logically_approximate.
+  split. admit. (* weakening *)
+  split. admit. (* weakening *)
+  intros k ρ γ γ' RD RG.
+  unfold LR_logically_approximate in H_approx_drop.
+  destruct_hypos.
+  assert (H_ty1 :
+    exists Tn, normalise (msubstT (msyn1 ρ) T) Tn /\
+      ([] ,, drop x Γ |-+ (msubstA (msyn1 ρ) e) : Tn)) by admit.
+  assert (H_ty2 :
+    exists Tn, normalise (msubstT (msyn2 ρ) T) Tn /\
+      ([] ,, drop x Γ |-+ (msubstA (msyn2 ρ) e') : Tn)) by admit.
+Admitted.
 
 
 Lemma compatibility_TyAbs: forall Delta Gamma bX K T e e',
@@ -25,7 +141,7 @@ Proof with eauto_LR.
   split... 
   split...
 
-  intros k rho env env' HRD HRG.
+  intros k rho γ γ' HRD HRG.
 
   autorewrite with RC.
 
@@ -93,13 +209,21 @@ Proof with eauto_LR.
   rewrite <- substA_msubstA by eauto using Ty.kindable_empty__closed.
   rewrite <- substA_msubstA by eauto using Ty.kindable_empty__closed.
 
+  apply drop_ty_var__RG with (bX := bX) in HRG as [γ_dropped [γ_dropped' H_RG']].
+  assert (HRD' : RD ((bX, K) :: Delta) ((bX, (Chi, T1, T2)) :: rho)). {
+    eauto using RD.
+  }
+  (*
+  specialize (IH__e _ _ _ _ HRD' H_RG').
   eapply IH__e.
   - eapply RD_cons; eauto.
   - apply RG_extend_rho.
     eapply RG_monotone; eauto.
     rewrite <- minus_n_O in Hlt_i.
+    assert (H_ : inclusion γ_dropped γ /\ inclusion γ_dropped' γ').
 
 
     (* apply Nat.lt_le_incl.
     assumption. *)
+    *)
 Admitted.
